

# № 9.1, 9.2, 10.1, 10.2

Демонстрация задания №10  
№9.1

$x_i \backslash y_j$	0	2	5	$P_{i*}$
0	0,1	0,2	0,2	0,5
4	0,3	0,2	0	0,5
$P_{*j}$	0,4	0,4	0,2	1

$X_i$	0	4	$\Sigma$
$P_i$	0,5	0,5	1

$y_j$	0	2	5	$\Sigma$
$P_j$	0,4	0,4	0,2	1

$$M_x = 0,5 \cdot 0 + 0,5 \cdot 4 = 2$$

$$M_y = 0,4 \cdot 0 + 0,4 \cdot 2 + 0,2 \cdot 5 = 1,8$$

$$\sigma_x = \sqrt{D_x}$$

$$\begin{aligned} D_x &= M_x^2 - (M_x)^2 = \\ &= 0,5 \cdot 0^2 + 0,5 \cdot 4^2 - 2^2 = \\ &= \cancel{0,8} \cdot 8 - 4 = 4 \end{aligned}$$

$$\sigma_x = 2$$

$$\sigma_y = \sqrt{D_y} = \sqrt{M_y^2 - (M_y)^2}$$

$$\begin{aligned} D_y &= 0,4 \cdot 0^2 + 0,4 \cdot 2^2 + 0,2 \cdot 5^2 - 1,8^2 = \\ &= 1,6 + 5 - 3,24 = 3,36 \end{aligned}$$

$$\sigma_y = 1,83$$

$$\sigma_y = \sqrt{3,56} = 1,853$$

$$r(\xi, \eta) = r_{\xi, \eta} = \frac{\text{cov}(\xi, \eta)}{\sigma_{\xi} \sigma_{\eta}}$$

$$\text{cov}(\xi, \eta) = M(\xi, \eta) - M_{\xi} \cdot M_{\eta}$$

$$\begin{aligned} \text{cov} &= M(\xi, \eta) - 2 \cdot 1,8 = \\ &= 1,6 - 3,6 = -2 \end{aligned}$$



$$\rho(x,y) = \frac{0,1 \cdot 0 \cdot 0}{\sqrt{0,2}} + 0,2 \cdot 0 \cdot 2 + 0,2 \cdot 0 \cdot 5 + 0,3 \cdot 0 \cdot 4 + 0,2 \cdot 2 \cdot 4 + 0,4 \cdot 5 = \frac{0,8}{1,833} = 0,436$$

$$\rho(x,y) = \frac{-2}{2 \cdot 1,833} = -0,5456$$

$\sqrt{0,2}$

	1	2	3	$P_{i*}$
1	$1/12$	$1/6$	$1/4$	$6/12$
2	$1/12$	$1/6$	$1/4$	$6/12$
$P_{*j}$	$2/12$	$2/6$	$2/4$	1

$$\begin{aligned} \text{COV}(x,y) &= M_{xy} - M_x M_y \\ M_y &= 1 \cdot 1 \cdot \frac{1}{12} + 1 \cdot 2 \cdot \frac{1}{6} + 1 \cdot 3 \cdot \frac{1}{4} + 2 \cdot 1 \cdot \frac{1}{12} + 2 \cdot 2 \cdot \frac{1}{6} + 2 \cdot 3 \cdot \frac{1}{4} = \end{aligned}$$

$$\rho(x,y) = \frac{\text{COV}(x,y)}{\sigma_x \sigma_y}$$

$$M_y = \frac{1}{12} + \frac{2}{6} + \frac{3}{4} + \frac{2}{12} + \frac{4}{6} + \frac{6}{4} =$$

$$= \frac{1}{12} + \frac{4}{12} + \frac{9}{12} + \frac{2}{12} + \frac{8}{12} + \frac{18}{12} =$$

$$= \frac{42}{12} = \frac{7}{2} = 3,5$$

$$M_x = \frac{6}{12} \cdot 1 + \frac{6}{12} \cdot 2 = \frac{18}{12} = 1,5$$

$$M_y = \frac{2}{12} \cdot 1 + \frac{2}{6} \cdot 2 + \frac{2}{4} \cdot 3 =$$

$$= \frac{2}{12} + \frac{8}{12} + \frac{18}{12} = \frac{28}{12} = 2,33$$

$$\text{cov}(x, y) = 1,5 - 1,5 \cdot 2,33 =$$

$$= 3,5 - 3,5 = 0$$

$$\sigma_x = \sqrt{D_x}$$

$$D_x = M_{x^2} - (M_x)^2 =$$

$$= \frac{6}{12} \cdot 1^2 + \frac{6}{12} \cdot 2^2 = \frac{6}{12} + \frac{24}{12} = 2,5 - 1,5^2 =$$

$$\sigma_x = \sqrt{2,5} = 1,5811$$

$$= 0,25$$

$$\sqrt{0,25} = 0,5$$

$$\sigma_y = \sqrt{D_y}$$

$$D_y = M_{y^2} - (M_y)^2 =$$

$$= \frac{2}{12} \cdot 1^2 + \frac{2}{6} \cdot 2^2 + \frac{2}{4} \cdot 3^2 - 2,33^2 =$$

$$= \frac{2}{12} + \frac{16}{12} + \frac{54}{12} - 5,4289 =$$



$$-5,4289 = 6 - 5,4289 >$$

$$= 0,5719$$

$$6y = 10,5719 = 0,7557$$

$$r(x,y) = \frac{-2}{0,5 \cdot 0,7557} = -5,2931$$

$$\cos(x,y) = 0 \Rightarrow r(x,y) = 0$$

no. 1

$$Y): f(x,y) = \begin{cases} a \cos x \cos y & (x,y) \in D \\ 0, & (x,y) \notin D \end{cases}$$

$$D: 0 \leq x \leq \frac{\pi}{2}$$

$$0 \leq y \leq \frac{\pi}{2}$$

$$f(x) = \int_{-\infty}^{+\infty} f(x,y) dy = \int_0^{\frac{\pi}{2}} a \cos x \cos y dy =$$

$$= a \cos x \cdot (-\sin y) \Big|_0^{\frac{\pi}{2}} = a \cos x \cdot (-\sin \frac{\pi}{2}) - 0$$

$$= -a \cos x$$

$$f(x) = \begin{cases} a \cos x, & x \in D \\ 0, & x \notin D \end{cases}$$

$$F(y) = \int_{-\infty}^{\infty} f(x, y) dx = \int_0^{\frac{\pi}{2}} a \cos x \cos y dx =$$

$$= a \cos y \cdot (\sin x) \Big|_0^{\frac{\pi}{2}} =$$

$$= a \cos y - 0$$

$$f(y) = \begin{cases} a \cos y, & y \in D \\ 0, & y \notin D \end{cases}$$

~~$$F(x) = \int_0^{\frac{\pi}{2}} a \cos x dx =$$~~
~~$$= -a \sin x \Big|_0^{\frac{\pi}{2}} = -a$$~~

~~$$F(y) = \int_0^{\frac{\pi}{2}} a \cos y dy = -a \sin y \Big|_0^{\frac{\pi}{2}} = -a$$~~



$$f(x) = \int f(x) dx = \begin{cases} \sin x, & x \in D \\ 0, & x \leq 0 \\ 1, & x > \frac{\pi}{2} \end{cases}$$

$$f(y) = \int f(y) dy = \begin{cases} \sin x, & x \in D \\ 0, & x \leq 0 \\ 1, & x > \frac{\pi}{2} \end{cases}$$

$$f(x,y) = \begin{cases} \frac{1}{10\pi}, & \frac{x^2}{25} + \frac{y^2}{4} \leq 1 \\ 0, & \frac{x^2}{25} + \frac{y^2}{4} > 1 \end{cases}$$

$$F(x) = \int_{-\infty}^{\infty} F(x,y) dy$$

$$\frac{y^2}{4} < 1 - \frac{x^2}{25} \Rightarrow y \in \left[ -2\sqrt{1 - \frac{x^2}{25}}, 2\sqrt{1 - \frac{x^2}{25}} \right]$$

$$\text{for } x \in [-5, 5]$$

$$\left( \frac{x^2}{25} \leq 1 \right)$$

$$F(x) = 0 \quad \text{for } x \notin [-5, 5]$$

$$f(x) = \int_{-\infty}^x f(x,y) dx$$

$$\frac{y^2}{4} \leq 1 \Rightarrow y \in [-2, 2]$$

$$\frac{x^2}{25} \leq 1 - \frac{y^2}{4} \Rightarrow x \in \left[-5\sqrt{1 - \frac{y^2}{4}}, 5\sqrt{1 - \frac{y^2}{4}}\right]$$

$$F(y) = \int_{-5\sqrt{1 - \frac{y^2}{4}}}^{5\sqrt{1 - \frac{y^2}{4}}} \frac{1}{10\pi} dx =$$

$$= \frac{1}{10\pi} \cdot 10\sqrt{1 - \frac{y^2}{4}} = \frac{1}{\pi} \sqrt{1 - \frac{y^2}{4}}$$

$$\text{para } y \in [-2; 2]$$

$$f(y) = 0 \text{ para } y \notin [-2; 2]$$

$$f(x) = \begin{cases} \frac{2}{5\pi} \sqrt{1 - \frac{x^2}{25}}, & x \in [-5, 5] \\ 0, & x \notin [-5, 5] \end{cases}$$

$$f(y) = \begin{cases} \frac{1}{\pi} \sqrt{1 - \frac{y^2}{4}}, & y \in [-2, 2] \\ 0, & y \notin [-2; 2] \end{cases}$$



# Дз № 9.3, 9.4, (10.3, 10.4)

№ 9.3

$x_i$	1	3
$p_i$	0,4	0,6

$y_j$	2	4
$p_j$	0,2	0,8

$X \backslash Y$	2	4	$P_{ix}$
1	0,08	0,32	0,4
3	0,12	0,48	0,6
$P_{xj}$	0,2	0,8	1

$$M_x = 1 \cdot 0,4 + 3 \cdot 0,6 = 2,2$$

$$M_y = 2 \cdot 0,2 + 4 \cdot 0,8 = 3,6 \geq 5,8$$

$$D(x+y) = D_x + D_y + 2 \cdot \text{cov}(x, y)$$

$$D_x = M_x^2 - (M_x)^2 = 1 \cdot 0,4 + 3^2 \cdot 0,6 - 2,2^2 = 0,4 + 5,4 - 4,84 = 0,96$$

$$D_y = M_y^2 - (M_y)^2 = 2^2 \cdot 0,2 + 4^2 \cdot 0,8 - 3,6^2 = 0,8 + 12,8 - 12,96 = 0,64$$

$$\begin{aligned} \text{cov}(x, y) &= M_{xy} - M_x \cdot M_y = \\ &= 1 \cdot 2 \cdot 0,08 + 1 \cdot 4 \cdot 0,32 + 3 \cdot 2 \cdot 0,12 + 3 \cdot 4 \cdot 0,48 - \\ &= 2,2 \cdot 3,6 = 7,92 - 7,92 = 0 \end{aligned}$$

$$D(x+y) = 0,08 + 0,64 + 2 \cdot \overset{0}{\cancel{(-0,36)}} = 1,0$$

~~$$D_{xy} = M_{xy}^2 - (M_{xy})^2 =$$

$$= 1^2 \cdot 2^2 \cdot 0,08 + 1^2 \cdot 4^2 \cdot 0,32 +$$

$$+ 3^2 \cdot 2^2 \cdot 0,12 + 3^2 \cdot 4^2 \cdot 0,48 - (7,92)^2 =$$

$$= 0,32 + 5,12 + 4,32 + 69,12 - 62,7264$$~~

$$P(1+2) = 0,08$$

$$P(1+4) = 0,32 \quad P(5) = 0,32 + 0,12 = 0,44$$

$$P(3+2) = 0,12$$

$$P(3+4) = 0,48$$

$x+y$	3	5	7
$p_i$	0,08	0,44	0,48

~~$$M_{xy} = 3 \cdot 0,08 + 5 \cdot 0,44 + 7 \cdot 0,48 =$$

$$= 0,24 + 2,2 + 3,36 = 5,8$$~~



$$\begin{aligned}
 D_{xy} &= M_{xy}^2 - M_{xy}^2 \\
 &= 5^2 \cdot 0,08 + 5^2 \cdot 0,44 + 7^2 \cdot 0,48 - 38^2 = \\
 &= 0,92 + 11 + 23,52 - 33,64 = \\
 &= 1,8
 \end{aligned}$$

~~$\sqrt{2/4}$~~

~~5 секунд      3 минут~~

<del>x \backslash y</del>	<del>0</del>	<del>1</del>	<del>2</del>	<del><math>P_{i*}</math></del>
<del>0</del>	<del>0</del>	<del>0</del>	<del><math>\frac{25}{64}</math></del>	<del><math>\frac{25}{64}</math></del>
<del>1</del>	<del>0</del>	<del><math>\frac{15}{64}</math></del>	<del>0</del>	<del><math>\frac{15}{64}</math></del>
<del>2</del>	<del><math>\frac{9}{64}</math></del>	<del>0</del>	<del>0</del>	<del><math>\frac{9}{64}</math></del>
<del><math>P_{*j}</math></del>	<del><math>\frac{9}{64}</math></del>	<del><math>\frac{15}{64}</math></del>	<del><math>\frac{25}{64}</math></del>	

$$(1,1) = \frac{5}{8} \cdot \frac{3}{8} = \frac{15}{64}$$

$$(0,2) = \frac{5}{8} \cdot \frac{5}{8} = \frac{25}{64}$$

$$P(0,2) = \frac{3}{8} \cdot \frac{3}{8} = \frac{9}{64}$$

$$\begin{aligned}
 C_8^2 &= \frac{8!}{2! \cdot 6!} = 28
 \end{aligned}$$

5 den  
y

3 runde  
x

1 2 4

x \ y	0	1	2	P <sub>x</sub>
0	0	0	$\frac{10}{28}$	$\frac{10}{28}$
1	0	$\frac{15}{28}$	0	$\frac{15}{28}$
2	$\frac{3}{28}$	0	0	$\frac{3}{28}$
P <sub>x</sub>	$\frac{3}{28}$	$\frac{15}{28}$	$\frac{10}{28}$	1

$$\binom{8}{8} = \frac{8!}{2! \cdot (8-2)!} = \frac{8!}{2! \cdot 6!} = 28$$

$$\binom{3}{3} = \frac{3!}{2! \cdot 1!} = \frac{3}{2}$$

$$P(0,2) = \frac{\binom{2}{5}}{\binom{2}{8}} = \frac{10}{28}$$

$$P(1,1) = \frac{\binom{1}{5} \cdot \binom{1}{3}}{\binom{1}{8}} =$$

$$= \frac{5!}{(5-1)! \cdot 1!} \cdot \frac{3!}{(3-1)! \cdot 1!} =$$

28

$$= \frac{5 \cdot 3}{28} = \frac{15}{28}$$



$$M_x = 0 \cdot \frac{3}{28} + 1 \cdot \frac{15}{28} + 2 \cdot \frac{10}{28} =$$

$$= \cancel{\frac{0}{28}} + \frac{15}{28} + \frac{20}{28} = \cancel{\frac{35}{28}} = \frac{5}{4}$$

$$M_y = 2 \cdot \frac{3}{28} + 1 \cdot \frac{15}{28} + 0 \cdot \frac{10}{28} =$$

$$= \frac{6}{28} + \frac{15}{28} + 0 = \frac{21}{28} = \frac{3}{4}$$

$$D_x = 0^2 + 1^2 \cdot \frac{15}{28} + 2^2 \cdot \frac{10}{28} - \left(\frac{5}{4}\right)^2 =$$

$$= \frac{15}{28} + \frac{40}{28} - \frac{25}{16} = \frac{55}{28} - \frac{25}{16} =$$

$$= 1,9643 - 1,5625 = \underline{0,4018}$$

$$D_y = 2^2 \cdot \frac{3}{28} + 1^2 \cdot \frac{15}{28} + 0^2 \cdot \frac{10}{28} - \left(\frac{3}{4}\right)^2 =$$

$$= \frac{12}{28} + \frac{15}{28} - \frac{9}{16} = \frac{27}{28} - \frac{9}{16} =$$

$$= 0,9643 - 0,5625 = \underline{0,4018}$$

$$Cov(x, y) = 0 \cdot 2 \cdot \frac{3}{28} + 1 \cdot 1 \cdot \frac{15}{28}$$

$$+ 2 \cdot 0 \cdot \frac{5}{14} - \frac{5 \cdot 3}{4} + \frac{15}{28} - \frac{15}{16}$$

$$= \frac{15}{28} - \frac{15}{16} = 0,5357 - 0,9375 =$$

$$= -0,4018$$

$$r_{xy} = \frac{-0,4018}{\sqrt{0,4018} \cdot \sqrt{0,4018}} = \frac{-0,4018}{0,4018} = -1$$